associating the other way for better notation

examples/asm/asm.fst
@@ -15,7 +15,8 @@ effect ASM (a:Type) (wp:ASM_WP a) = ASM_ a wp wp  //we'll use this one instead
 effect Asm (a:Type) (pre:ASM_Pre) (post: (reg -> ASM_Post a)) = //and this one, which is more like a Hoare triple
        ASM_ a
              (fun (p:ASM_Post a) (h:reg) -> pre h /\ (forall a h1. (pre h /\ post h a h1) ==> p a h1)) (* WP *)
-             (fun (p:ASM_Post a) (h:reg) -> (forall a h1. (pre h /\ post h a h1) ==> p a h1))         (* WLP *)
+             (fun (p:ASM_Post a) (h:reg) -> pre h /\ (forall a h1. (pre h /\ post h a h1) ==> p a h1)) (* WP *)
+             (* (fun (p:ASM_Post a) (h:reg) -> (forall a h1. (pre h /\ post h a h1) ==> p a h1))         (\* WLP *\) *)
 
 
 type instr = 
@@ -33,6 +34,9 @@ type prog = list instr
 val finished : unit -> ASM prog  (fun (post:ASM_Post prog) (r0:reg) -> post [] r0)
 let finished _ = []
 
+val nop : unit -> ASM prog  (fun (post:ASM_Post prog) (r0:reg) -> post [] r0)
+let nop _ = []
+
 
 type ASMComp (wp:ASM_WP prog) = unit -> ASM prog wp
 type AsmComp (pre:ASM_Pre) (post:reg -> ASM_Post prog) = unit -> Asm prog pre post
@@ -45,20 +49,33 @@ assume val op_Hat_Hat : #wp:ASM_WP prog
 
 val add_2: AsmComp (requires (fun r -> True))
 		  (ensures (fun r_0 p r_1 -> r_1 = r_0 + 2))
-let add_2 =  //regardless of the associativity of  >>, you currently need the parenthesis because of the precedence of function application
-       Add 1  
-   ^^ (Add 1
-   ^^ finished)
+let add_2 =  //^^ associates the wrong way, unfortunately
+       (Add 1  
+    ^^ (Add 1
+    ^^ finished))
+
+//we could define an operator that sequences in the other direction, a snoc instead of a cons
+assume val op_Hat_Bar : #wp:ASM_WP prog
+	       -> =f:ASMComp wp
+      	       -> i:instr 
+	       -> Tot (ASMComp (fun (post:ASM_Post prog) (r0:reg) -> 
+			      wp (fun p r1 -> post (List.append p [i]) (eval i r1)) r0))
+val add_3: AsmComp (requires (fun r -> True))
+		  (ensures (fun r_0 p r_1 -> r_1 = r_0 + 3))
+let add_3 = nop
+    ^| (Add 1)
+    ^| (Add 1)
+    ^| (Add 1)
+
 
 val add_4: AsmComp 
   (requires (fun r -> True))
   (ensures (fun r_0 p r_1 -> r_1 = r_0 + 4))
-let add_4 = 
-      Add 2
-  ^^ (Add 2
-  ^^ (Add 2 
-  ^^ (Sub 2
-  ^^  finished)))
+let add_4 = nop
+  ^| (Add 2)
+  ^| (Add 2)
+  ^| (Add 2)
+  ^| (Sub 2)
 
 (* Composing two basic blocks in sequence *)
 assume val op_Hat_Hat_Hat : 
